NLustre/NLSemantics.v
@@ -351,7 +351,7 @@ environment.
           sem_laexps bk H ck arg ls ->
           sem_vars bk H x xs ->
           sem_var bk H y ys ->
-          sem_reset f (reset_of ys) ls xs ->
+          sem_reset f (reset_of ys) (map (fun _ => absent) arg) ls (map (fun _ => absent) x) xs ->
           sem_equation bk H (EqApp x ck f arg (Some y))
     | SEqFby:
         forall bk H x ls xs c0 ck le,
@@ -360,11 +360,11 @@ environment.
           xs = fby (sem_const c0) ls ->
           sem_equation bk H (EqFby x ck c0 le)
 
-    with sem_reset: ident -> stream bool -> stream (list value) -> stream (list value) -> Prop :=
+    with sem_reset: ident -> stream bool -> list value -> stream (list value) -> list value -> stream (list value) -> Prop :=
          | SReset:
-             forall f r xss yss,
-               (forall n, sem_node f (mask_vs n r xss) (mask_vs n r yss)) ->
-               sem_reset f r xss yss
+             forall f r opaque_x xss opaque_y yss,
+               (forall n, sem_node f (mask opaque_x n r xss) (mask opaque_y n r yss)) ->
+               sem_reset f r opaque_x xss opaque_y yss
 
     with sem_node: ident -> stream (list value) -> stream (list value) -> Prop :=
          | SNode:
@@ -400,7 +400,7 @@ enough: it does not support the internal fixpoint introduced by
     Variable G: global.
 
     Variable P_equation: stream bool -> history -> equation -> Prop.
-    Variable P_reset: ident -> stream bool -> stream (list value) -> stream (list value) -> Prop.
+    Variable P_reset: ident -> stream bool -> list value -> stream (list value) -> list value -> stream (list value) -> Prop.
     Variable P_node: ident -> stream (list value) -> stream (list value) -> Prop.
 
     Hypothesis EqDefCase:
@@ -422,8 +422,8 @@ enough: it does not support the internal fixpoint introduced by
         sem_laexps bk H ck arg ls ->
         sem_vars bk H x xs ->
         sem_var bk H y ys ->
-        sem_reset G f (reset_of ys) ls xs ->
-        P_reset f (reset_of ys) ls xs ->
+        sem_reset G f (reset_of ys) (map (fun _ => absent) arg) ls (map (fun _ => absent) x) xs ->
+        P_reset f (reset_of ys) (map (fun _ => absent) arg) ls (map (fun _ => absent) x) xs ->
         P_equation bk H (EqApp x ck f arg (Some y)).
 
     Hypothesis EqFbyCase:
@@ -434,10 +434,10 @@ enough: it does not support the internal fixpoint introduced by
         P_equation bk H (EqFby x ck c0 le).
 
     Hypothesis ResetCase:
-      forall f r xss yss,
-        (forall n, sem_node G f (mask_vs n r xss) (mask_vs n r yss)) ->
-        (forall n, P_node f (mask_vs n r xss) (mask_vs n r yss)) ->
-        P_reset f r xss yss.
+      forall f r opaque_x xss opaque_y yss,
+        (forall n, sem_node G f (mask opaque_x n r xss) (mask opaque_y n r yss)) ->
+        (forall n, P_node f (mask opaque_x n r xss) (mask opaque_y n r yss)) ->
+        P_reset f r opaque_x xss opaque_y yss.
 
     Hypothesis NodeCase:
       forall bk H f xss yss n, (* i o v eqs ingt0 outgt0 defd vout nodup good, *)
@@ -463,9 +463,11 @@ enough: it does not support the internal fixpoint introduced by
             (Sem: sem_equation G b H e) {struct Sem}
       : P_equation b H e
     with sem_reset_mult
-           (f: ident) (r: stream bool) (xss oss: stream (list value))
-           (Sem: sem_reset G f r xss oss) {struct Sem}
-         : P_reset f r xss oss
+           (f: ident) (r: stream bool)
+           (opaque_x: list value) (xss: stream (list value))
+           (opaque_o: list value) (oss: stream (list value))
+           (Sem: sem_reset G f r opaque_x xss opaque_o oss) {struct Sem}
+         : P_reset f r opaque_x xss opaque_o oss
     with sem_node_mult
            (f: ident) (xss oss: stream (list value))
            (Sem: sem_node G f xss oss) {struct Sem}
@@ -857,8 +859,8 @@ clock to [sem_var_instant] too. *)
                         using sem_node_mult
       with (P_equation := fun bk H eq => ~Is_node_in_eq node.(n_name) eq
                                       -> sem_equation G bk H eq)
-           (P_reset := fun f r xss yss => node.(n_name) <> f ->
-                                       sem_reset G f r xss yss).
+           (P_reset := fun f r opaque_x xss opaque_y yss => node.(n_name) <> f ->
+                                                         sem_reset G f r opaque_x xss opaque_y yss).
     - econstructor; eassumption.
     - intro Hnin.
       eapply @SEqApp with (1:=Hlae) (2:=Hvars).
@@ -1130,6 +1132,76 @@ an absent value *)
     - inv Hsem; auto.
     - inversion_clear Hsem as [|? ? ? Heqs'].
       inv Heqs'; auto.
+  Qed.
+
+  (** Morphisms properties *)
+
+  Lemma clock_of_compat:
+    forall xs xs' bk,
+      (forall n, xs n = xs' n) ->
+      clock_of xs bk ->
+      clock_of xs' bk.
+  Proof.
+    unfold clock_of. intros ** E Pres n.
+    split; intros H.
+    - apply Pres.
+      specialize (E n).
+      induction H; rewrite E; constructor; auto.
+    - apply Pres in H.
+      specialize (E n).
+      induction H; rewrite <-E; constructor; auto.
+  Qed.
+
+  Lemma sem_vars_compat:
+    forall H bk x xs xs',
+      (forall n, xs n = xs' n) ->
+      sem_vars bk H x xs ->
+      sem_vars bk H x xs'.
+  Proof.
+    unfold sem_vars, lift; intros ** E Sem n.
+    specialize (E n); specialize (Sem n).
+    induction Sem; rewrite <-E; constructor; auto.
+  Qed.
+
+  Lemma same_clock_compat:
+    forall xs xs',
+      (forall n, xs n = xs' n) ->
+      same_clock xs ->
+      same_clock xs'.
+  Proof.
+    unfold same_clock; intros ** E ? ?; rewrite <-E; auto.
+  Qed.
+
+ Lemma sem_node_compat:
+    forall G f xss xss' yss yss',
+      (forall n, xss n = xss' n) ->
+      (forall n, yss n = yss' n) ->
+      sem_node G f xss yss ->
+      sem_node G f xss' yss'.
+  Proof.
+    intros ** Exss Eyss Node.
+    inv Node.
+    econstructor; eauto.
+    - eapply clock_of_compat; eauto.
+    - eapply sem_vars_compat; eauto.
+    - eapply sem_vars_compat; eauto.
+    - eapply same_clock_compat; eauto.
+    - eapply same_clock_compat; eauto.
+    - intro; rewrite <-Exss, <-Eyss; auto.
+  Qed.
+
+  Corollary sem_reset_compat:
+    forall G f r r' opaque_x xss opaque_o oss,
+      (forall n, r n = r' n) ->
+      sem_reset G f r opaque_x xss opaque_o oss ->
+      sem_reset G f r' opaque_x xss opaque_o oss.
+  Proof.
+    intros ** E Res.
+    inversion_clear Res as [? ? ? ? Node].
+    constructor; intro n.
+    pose proof (mask_compat _ _ n opaque_x xss E).
+    pose proof (mask_compat _ _ n opaque_o oss E).
+    eapply sem_node_compat; eauto.
   Qed.
 
 End NLSEMANTICS.
